LeanOS.lean
@@ -1,2 +1,4 @@
 import LeanOS.Kernel
 import LeanOS.Proofs
+import LeanOS.Arm
+import LeanOS.Tables
